lakefile.lean
@@ -5,8 +5,8 @@ package «reflection» {
   -- add package configuration options here
 }
 
-require std from git "https://github.com/leanprover/std4" @ "nightly-testing-2024-04-04"
-require aesop from git "https://github.com/JLimperg/aesop" @ "5fefb40a7c9038a7150e7edd92e43b1b94c49e79"
+-- require std from git "https://github.com/leanprover/std4" @ "nightly-testing-2024-04-04"
+-- require aesop from git "https://github.com/JLimperg/aesop" @ "master"
 -- require IIT from git "https://github.com/arthur-adjedj/iit" @ "v4.4.0"
 require Qq from git "https://github.com/leanprover-community/quote4"
 -- require mathlib from git "https://github.com/leanprover-community/mathlib4"
